---
layout: post
title:   test 10
date:   2019-6-16 00:00:01 +09:00
author: "장재혁"
categories: zkp
tag: [zkp]
youtubeId :
slideWebId :
---
$$
\begin{align}
(x+y)^3&=(x+y)(x+y)^2\\
       &=(x+y)(x^2+2xy+y^2)\\
       &=x^3+3x^2y+3xy^3+x^3.\qedhere
\end{align}
$$

 $$\Pr j$$


$$\operatorname{d}\!y\over\operatorname{d}\!x$$


$$\sqrt[3]{x^3+y^3 \over 2}$$

$$_{n}\mathrm{H}_{k}, P(n,k)$$

$$dy \over dx$$

$$\nleftrightarrow$$

$$\dot{a}$$

$$ \left\{ {\left[ \frac{\beta v_i\left( x \right)+\alpha w_i\left( x \right)+y_i\left( x \right)}{\gamma } \right]}_G \right\}_{i=m-1}^{m}$$

$$ \left\{ {\left[ {x^i} \right]}_G \right\}_{i=0}^{n-1} $$

$$ \left\{ {\left[ \frac{x^i t(x)}{\delta } \right]}_G \right\}_{i=0}^{n-2}$$

$$dy \over dx$$



$$\sigma _H:=( \left [ \beta \right]_H, \left[ \gamma \right]_H, \left[ \delta \right]_H, \left\{ {\left[ {x^i} \right]}_H \right\}_{i=0}^{n-1} )$$

$$\left[ A \right]_G:= \left[ \alpha \right]_G +\sum\nolimits_{i=1}^m c_i \sum\nolimits_{k=0}^{n-1} a_{i,k} {\left[ {x^k} \right]}_G + r{\left[ \delta \right]}_G$$

$$\sum\nolimits_{i=1}^m c_i$$

$$\left[ B \right]_H:= \left[ \beta \right]_H + \sum\nolimits_{i=1}^m c_i \sum\nolimits_{k=0}^{n-1} b_{i,k} {\left[ {x^k} \right]}_H + s{\left[ \delta \right]}_H$$

$$\sum\nolimits_{k=0}^{n-2} d_k {\left[ \frac{x^k t(x)}{\delta } \right]}_G$$

$${\left[ C \right]}_G:=\sum\nolimits_{i=1}^{i=m-2} c_i{\left[ \frac{\beta v_i(x)+\alpha w_i (x) + y_i (x)}{ \delta } \right]}_G + \sum\nolimits_{k=0}^{n-2} d_k {\left[ \frac{x^k t(x)}{\delta } \right]}_G + s{\left[ A \right]}_G + r{\left[ B \right]}_G - rs{\left[ \delta \right]}_G$$

$${\left[ C \right]}_G$$

$$\sum\nolimits_{i=1}^{i=m-2} c_i{\left[ \frac{\beta v_i(x)+\alpha w_i (x) + y_i (x)}{ \delta } \right]}_G$$


$$
LHS = {\left[ A \right]}_G \cdot {\left[ B \right]}_H = {\left [ \alpha + \sum\nolimits_{i=1}^{m} c_i v_i(x) + r\delta \right]}_G \cdot {\left [ \beta + \sum\nolimits_{i=1}^{m} c_i w_i ( x ) + s \delta \right]}_H
$$

$$
= { \left [ \alpha \beta + \sum\nolimits_{i=1}^{m} c_i v_i ( x ) \cdot  \sum\nolimits_{i=1}^{m} c_i w_i ( x ) + ( \alpha + r \delta ) \sum\nolimits_{i=1}^{m} c_i w_i ( x ) + ( \beta +s\delta ) \sum\nolimits_{i=1}^{m} c_i v_i ( x )+ \alpha s \delta + \beta r \delta + r s {\delta }^{2} \right]}_{G\cdot H}
$$.

$$
RHS = { \left [ \alpha \right]}_G \cdot { \left [ \beta \right]}_H + ( \sum\nolimits_{i=m-1}^{m} c_i { \left [ \frac { \beta v_i ( x ) + \alpha w_i ( x ) + y_i ( x ) }{ \gamma } \right]}_G ) \cdot { \left [ \gamma \right]}_H + { \left [ C \right]}_G \cdot { \left [ \delta \right]}_H
$$



$$
{ \left [A' \right]}_G := { \left [ \alpha \right]}_G + { \left [ V \right]}_G + { \left [ \sum\nolimits_{i=m-1}^{m} c_i v_i ( x ) \right]}_G + r { \left [ \delta \right]}_G
$$

$$
{ \left [B' \right]}_H := { \left [ \beta \right]}_H + { \left [ W \right]}_H + { \left [ \sum\nolimits_{i=m-1}^{m} c_i w_i ( x ) \right]}_H + s{ \left [ \delta \right]}_H
$$

$$
{ \left [ C' \right]}_G := { \left [ \frac { ( \beta V + \alpha W + Y )}{ \delta } \right]}_G + { \left [ \frac { t ( x ) H }{ \delta } \right]}_G + s { \left [
A' \right]}_G + r { \left [ B' \right]}_G - rs{ \left [ \delta \right]}_G
$$

$$
\sigma _G:= \begin{Bmatrix} \left [ \alpha \right]_G, \left[ \beta \right]_G,\left[ \delta \right]_G, \left\{ {\left[ {x^i} \right]}_G \right\}_{i=0}^{n-1}, 
\\ \left\{ {\left[ \frac{\beta v_i\left( x \right)+\alpha w_i\left( x \right)+y_i\left( x \right)}{\gamma } \right]}_G \right\}_{i=m-1}^{m},
\\ \left\{ {\left[ \frac{\beta v_i\left( x \right)+\alpha w_i\left( x \right)+y_i\left( x \right)}{\delta } \right]}_G \right\}_{i=1}^{m-2}, 
\\ \left\{ {\left[ \frac{x^i t(x)}{\delta } \right]}_G \right\}_{i=0}^{n-2}& \\ \end{Bmatrix}
$$

$$
\pi ' =  \begin{pmatrix} { \left [ [A' \right]}_G := { \left [ \alpha \right]}_G + { \left [ V \right]}_G + { \left [ \sum\nolimits_{i=m-1}^{m} c_i v_i ( x ) \right]}_G + r { \left [ \delta \right]}_G, \\
{ \left [B' \right]}_H := { \left [ \beta \right]}_H + { \left [ W \right]}_H + { \left [ \sum\nolimits_{i=m-1}^{m} c_i w_i ( x ) \right]}_H + s{ \left [ \delta \right]}_H, \\
{ \left [ C' \right]}_G := { \left [ \frac { ( \beta V + \alpha W + Y )}{ \delta } \right]}_G + { \left [ \frac { t ( x ) H }{ \delta } \right]}_G + s { \left [
A' \right]}_G + r { \left [ B' \right]}_G - rs{ \left [ \delta \right]}_G \\
\end{pmatrix} 
$$

$$
s_N{ \left [A_N \right]}_G - r_N { \left [ B_N \right]}_G - {\left[ r_N s_N \delta_N} \right]}_G

$$ 
{ \left [ \frac { h ( x_N ) t ( x_N )}{ \delta_N } \right]}_G = { \left [ C_N \right]}_G - \sum\nolimits_{i=1}^{i=m-2} \frac { ( \beta_N v_i ( x_N ) + \alpha_N w_i ( x_N ) + y_i ( x_N ) ) }{\delta_N} { \left [ c_i \right]}_G - s_N{ \left [A_N \right]}_G - r_N { \left [ B_N \right]}_G - {\left[ r_N s_N \delta_N \right]}_G
$$

$$ 
\pi ' = \begin{pmatrix} { \left [ A' \right]}_G := { \left [ \alpha +r \delta \right]}_G + \sum\nolimits_{i=1}^{m} v_i ( x_N ) { \left [ c_i \right]}_G, \\ { \left [ B ' \right]}_H = { \left [ \beta + s \delta \right]}_H + \sum\nolimits_{i=1}^{m} w_i ( x_N ) { \left [ c_i \right]}_H, \\ { \left [ C ' \right]}_G = \sum\nolimits_{i=1}^{i=m} \frac { ( \beta v_i ( x_N ) + \alpha w_i ( x_N ) + y_i ( x_N ) ) }{ \delta }{ \left [ c_i \right]}_G - \sum\nolimits_{i=m-1}^{i=m} \frac{ ( \beta v_i ( x ) + \alpha w_i ( x ) + y_i ( x ) )}{ \delta }{ \left [ c_i \right]}_G \\  +\frac { {\left [ h ( x_N ) t ( x_N ) \right]}_G}{ \delta } + { \left [ s A '+ r B ' - r s \delta \right]}_G \\
\end{pmatrix}
$$. 

$$
+\frac { {\left [ h ( x_N ) t ( x_N ) \right]}_G}{ \delta } + { \left [ s A '+ r B ' - r s \delta \right]}_G
$$

$$
\begin{bmatrix}
\quad \\
\mathbf{R} \\
\quad
\end{bmatrix}^T

\begin{bmatrix}
\quad & \quad & \quad \\
\quad & \mathbf{A} & \quad \\
\quad & \quad & \quad
\end{bmatrix}_{m \times n} \cdot

\begin{bmatrix}
\quad \\
\mathbf{R} \\
\quad
\end{bmatrix}^T

\begin{bmatrix}
\quad & \quad & \quad \\
\quad & \mathbf{B} & \quad \\
\quad & \quad & \quad
\end{bmatrix}
=
\begin{bmatrix}
\quad \\
\mathbf{R} \\
\quad
\end{bmatrix}^T
\begin{bmatrix}
\quad & \quad & \quad \\
\quad & \mathbf{C} & \quad \\
\quad & \quad & \quad
\end{bmatrix}
$$

$$
\begin{bmatrix} 1 & 2 \end{bmatrix} \cdot \begin{bmatrix} 3 & 4 \end{bmatrix} =  \begin{bmatrix}  3 & 8 \end{bmatrix}
$$

$$
\begin{bmatrix} 1 & 2 \end{bmatrix}
$$

$$\underbrace{h_t = qE_tx_t}_{\text{(the Schaefer production function)}}$$

$$
\begin{bmatrix} \quad \\ \mathbf{R} \\ \quad \end{bmatrix}^T \underbrace{ \begin{bmatrix} \quad & \quad & \quad \\ \quad & \mathbf{A} & \quad \\ \quad & \quad & \quad \end{bmatrix}}_{\text{m x n}} \cdot \begin{bmatrix} \quad \\ \mathbf{R} \\ \quad \end {bmatrix}^T \begin{bmatrix} \quad & \quad & \quad \\ \quad & \mathbf{B} & \quad \\
 \quad & \quad & \quad \end{bmatrix} = \begin{bmatrix} \quad \\ \mathbf{R} \\ \quad \end{bmatrix}^T \begin{bmatrix} \quad & \quad & \quad \\ \quad & \mathbf{C} & \quad \\ \quad & \quad & \quad \end{bmatrix}
$$




| Priority apples | Second priority | Third priority |
|-------|--------|---------|
| ambrosia | gala | red delicious |
| pink lady | jazz | macintosh |
| honeycrisp | granny smith | fuji |

|                                         |                                                 |
| --------------------------------------- | ------------------------------------------------ |
| ![](/images/article_9/media/image1.png){: width="100%" height="100%"} | ![](/images/article_9/media/image2.png){: width="100%" height="100%"} |

$$
\begin{tabular} {c} \hline
번호 & 항목 & 내용 \\ \hline \hline
1 & 차종 & 엑셀 \\
2 & 년식 & 1994 \\
3 & 배기량 & 1498 cc \\ \hline
\end{tabular}
$$